ci: more ink smart contracts to the Rust list of files

examples/ink_contracts/conditional_compilation.rs
@@ -1,0 +1,130 @@
+#[derive(Default, Clone, Copy)]
+struct AccountId(u128);
+
+type Balance = u128;
+
+type BlockNumber = u32;
+
+struct Env {
+    caller: AccountId,
+}
+
+impl Env {
+    fn caller(&self) -> AccountId {
+        self.caller
+    }
+
+    fn emit_event(&self, _event: Event) {
+        unimplemented!()
+    }
+
+    fn block_number(&self) -> BlockNumber {
+        unimplemented!()
+    }
+}
+
+pub trait Flip {
+    /// Flips the current value of the Flipper's boolean.
+    fn flip(&mut self);
+
+    /// Returns the current value of the Flipper's boolean.
+    fn get(&self) -> bool;
+
+    fn push_foo(&mut self, value: bool);
+}
+
+/// Feature gated event
+pub struct Changes {
+    // attributing event field with `cfg` is not allowed
+    new_value: bool,
+    by: AccountId,
+}
+
+/// Feature gated event
+pub struct ChangesDated {
+    // attributing event field with `cfg` is not allowed
+    new_value: bool,
+    by: AccountId,
+    when: BlockNumber,
+}
+
+enum Event {
+    Changes(Changes),
+    ChangesDated(ChangesDated),
+}
+
+pub struct ConditionalCompilation {
+    value: bool,
+}
+
+impl ConditionalCompilation {
+    fn init_env() -> Env {
+        unimplemented!()
+    }
+
+    fn env(&self) -> Env {
+        Self::init_env()
+    }
+
+    /// Creates a new flipper smart contract initialized to `false`.
+    pub fn new() -> Self {
+        Self {
+            value: Default::default(),
+        }
+    }
+
+    /// Constructor that is included when `foo` is enabled
+    pub fn new_foo(value: bool) -> Self {
+        Self { value }
+    }
+
+    /// Constructor that is included when `bar` is enabled
+    pub fn new_bar(value: bool) -> Self {
+        Self { value }
+    }
+
+    /// Constructor that is included with either `foo` or `bar` features enabled
+    pub fn new_foo_bar(value: bool) -> Self {
+        Self { value }
+    }
+
+    pub fn inherent_flip_foo(&mut self) {
+        self.value = !self.value;
+        let caller = Self::init_env().caller();
+        Self::init_env().emit_event(Event::Changes(Changes {
+            new_value: self.value,
+            by: caller,
+        }));
+    }
+
+    pub fn inherent_flip_bar(&mut self) {
+        let caller = Self::init_env().caller();
+        let block_number = Self::init_env().block_number();
+        self.value = !self.value;
+        Self::init_env().emit_event(Event::ChangesDated(ChangesDated {
+            new_value: self.value,
+            by: caller,
+            when: block_number,
+        }));
+    }
+}
+
+impl Flip for ConditionalCompilation {
+    fn flip(&mut self) {
+        self.value = !self.value;
+    }
+
+    fn get(&self) -> bool {
+        self.value
+    }
+
+    /// Feature gated mutating message
+    fn push_foo(&mut self, value: bool) {
+        let caller = Self::init_env().caller();
+        Self::init_env().emit_event(Event::Changes(Changes {
+            new_value: value,
+            by: caller,
+        }));
+        self.value = value;
+    }
+}
