examples/ink_contracts/contract_transfer.rs
@@ -1,0 +1,80 @@
+#[derive(Default, Clone, Copy)]
+struct AccountId(u128);
+
+type Balance = u128;
+
+struct Env {
+    caller: AccountId,
+}
+
+impl Env {
+    fn caller(&self) -> AccountId {
+        self.caller
+    }
+
+    fn balance(&self) -> Balance {
+        unimplemented!()
+    }
+
+    fn transfer(&mut self, _to: AccountId, _value: Balance) -> Result<(), ()> {
+        unimplemented!()
+    }
+
+    fn transferred_value(&self) -> Balance {
+        unimplemented!()
+    }
+}
+
+/// No storage is needed for this simple contract.
+pub struct GiveMe {}
+
+impl GiveMe {
+    fn init_env() -> Env {
+        unimplemented!()
+    }
+
+    fn env(&self) -> Env {
+        Self::init_env()
+    }
+
+    /// Creates a new instance of this contract.
+    pub fn new() -> Self {
+        Self {}
+    }
+
+    /// Transfers `value` amount of tokens to the caller.
+    ///
+    /// # Errors
+    ///
+    /// - Panics in case the requested transfer exceeds the contract balance.
+    /// - Panics in case the requested transfer would have brought this contract's
+    ///   balance below the minimum balance (i.e. the chain's existential deposit).
+    /// - Panics in case the transfer failed for another reason.
+    pub fn give_me(&mut self, value: Balance) {
+        println!("requested value: {}", value);
+        println!("contract balance: {}", self.env().balance());
+
+        assert!(value <= self.env().balance(), "insufficient funds!");
+
+        if self.env().transfer(self.env().caller(), value).is_err() {
+            panic!(
+                "requested transfer failed. this can be the case if the contract does not\
+                 have sufficient free funds or if the transfer would have brought the\
+                 contract's balance below minimum balance."
+            )
+        }
+    }
+
+    /// Asserts that the token amount sent as payment with this call
+    /// is exactly `10`. This method will fail otherwise, and the
+    /// transaction would then be reverted.
+    ///
+    /// # Note
+    ///
+    /// The method needs to be annotated with `payable`; only then it is
+    /// allowed to receive value as part of the call.
+    pub fn was_it_ten(&self) {
+        println!("received payment: {}", self.env().transferred_value());
+        assert!(self.env().transferred_value() == 10, "payment was not ten");
+    }
+}
