examples/ink_contracts/custom_environment.rs
@@ -1,0 +1,57 @@
+#[derive(Default, Clone, Copy)]
+struct AccountId(u128);
+
+type Balance = u128;
+
+struct Env {
+    caller: AccountId,
+}
+
+impl Env {
+    fn caller(&self) -> AccountId {
+        self.caller
+    }
+
+    fn emit_event(&self, _event: Event) {
+        unimplemented!()
+    }
+}
+
+/// Trivial contract with a single message that emits an event with many topics.
+#[derive(Default)]
+pub struct Topics;
+
+/// An event that would be forbidden in the default environment, but is completely
+/// valid in our custom one.
+#[derive(Default)]
+pub struct EventWithTopics {
+    first_topic: Balance,
+    second_topic: Balance,
+    third_topic: Balance,
+    fourth_topic: Balance,
+    fifth_topic: Balance,
+}
+
+enum Event {
+    EventWithTopics(EventWithTopics),
+}
+
+impl Topics {
+    fn init_env() -> Env {
+        unimplemented!()
+    }
+
+    fn env(&self) -> Env {
+        Self::init_env()
+    }
+
+    pub fn new() -> Self {
+        Default::default()
+    }
+
+    /// Emit an event with many topics.
+    pub fn trigger(&mut self) {
+        self.env()
+            .emit_event(Event::EventWithTopics(EventWithTopics::default()));
+    }
+}
