examples/ink_contracts/dns.rs
@@ -1,0 +1,242 @@
+#[derive(Default)]
+struct Mapping<K, V> {
+    _key: core::marker::PhantomData<K>,
+    _value: core::marker::PhantomData<V>,
+}
+
+impl<K, V> Mapping<K, V> {
+    fn contains(&self, _key: &K) -> bool {
+        unimplemented!()
+    }
+
+    fn get(&self, _key: &K) -> Option<V> {
+        unimplemented!()
+    }
+
+    fn insert(&mut self, _key: K, _value: V) -> Option<u32> {
+        unimplemented!()
+    }
+
+    fn new() -> Mapping<K, V> {
+        unimplemented!()
+    }
+
+    fn remove(&self, _key: K) {
+        unimplemented!()
+    }
+
+    fn size(&self, _key: K) -> Option<u32> {
+        unimplemented!()
+    }
+
+    fn take(&self, _key: K) -> Option<V> {
+        unimplemented!()
+    }
+}
+
+#[derive(Default, Clone, Copy, PartialEq)]
+struct AccountId(u128);
+
+impl std::convert::From<[u8; 32]> for AccountId {
+    fn from(_value: [u8; 32]) -> Self {
+        unimplemented!()
+    }
+}
+
+type Balance = u128;
+
+type Hash = [u8; 32];
+
+struct Env {
+    caller: AccountId,
+}
+
+impl Env {
+    fn caller(&self) -> AccountId {
+        self.caller
+    }
+
+    fn emit_event(&self, _event: Event) {
+        unimplemented!()
+    }
+}
+
+/// Emitted whenever a new name is being registered.
+pub struct Register {
+    name: Hash,
+    from: AccountId,
+}
+
+/// Emitted whenever an address changes.
+pub struct SetAddress {
+    name: Hash,
+    from: AccountId,
+    old_address: Option<AccountId>,
+    new_address: AccountId,
+}
+
+/// Emitted whenever a name is being transferred.
+pub struct Transfer {
+    name: Hash,
+    from: AccountId,
+    old_owner: Option<AccountId>,
+    new_owner: AccountId,
+}
+
+enum Event {
+    Register(Register),
+    SetAddress(SetAddress),
+    Transfer(Transfer),
+}
+
+/// Domain name service contract inspired by
+/// [this blog post](https://medium.com/@chainx_org/secure-and-decentralized-polkadot-domain-name-system-e06c35c2a48d).
+///
+/// # Note
+///
+/// This is a port from the blog post's ink! 1.0 based version of the contract
+/// to ink! 2.0.
+///
+/// # Description
+///
+/// The main function of this contract is domain name resolution which
+/// refers to the retrieval of numeric values corresponding to readable
+/// and easily memorable names such as "polka.dot" which can be used
+/// to facilitate transfers, voting and DApp-related operations instead
+/// of resorting to long IP addresses that are hard to remember.
+pub struct DomainNameService {
+    /// A hashmap to store all name to addresses mapping.
+    name_to_address: Mapping<Hash, AccountId>,
+    /// A hashmap to store all name to owners mapping.
+    name_to_owner: Mapping<Hash, AccountId>,
+    /// The default address.
+    default_address: AccountId,
+}
+
+impl Default for DomainNameService {
+    fn default() -> Self {
+        let mut name_to_address = Mapping::new();
+        name_to_address.insert(Hash::default(), zero_address());
+        let mut name_to_owner = Mapping::new();
+        name_to_owner.insert(Hash::default(), zero_address());
+
+        Self {
+            name_to_address,
+            name_to_owner,
+            default_address: zero_address(),
+        }
+    }
+}
+
+/// Errors that can occur upon calling this contract.
+#[derive(Debug, PartialEq, Eq)]
+pub enum Error {
+    /// Returned if the name already exists upon registration.
+    NameAlreadyExists,
+    /// Returned if caller is not owner while required to.
+    CallerIsNotOwner,
+}
+
+/// Type alias for the contract's result type.
+pub type Result<T> = core::result::Result<T, Error>;
+
+impl DomainNameService {
+    fn init_env() -> Env {
+        unimplemented!()
+    }
+
+    fn env(&self) -> Env {
+        Self::init_env()
+    }
+
+    /// Creates a new domain name service contract.
+    pub fn new() -> Self {
+        Default::default()
+    }
+
+    /// Register specific name with caller as owner.
+    pub fn register(&mut self, name: Hash) -> Result<()> {
+        let caller = self.env().caller();
+        if self.name_to_owner.contains(&name) {
+            return Err(Error::NameAlreadyExists);
+        }
+
+        self.name_to_owner.insert(name, caller);
+        self.env()
+            .emit_event(Event::Register(Register { name, from: caller }));
+
+        Ok(())
+    }
+
+    /// Set address for specific name.
+    pub fn set_address(&mut self, name: Hash, new_address: AccountId) -> Result<()> {
+        let caller = self.env().caller();
+        let owner = self.get_owner_or_default(name);
+        if caller != owner {
+            return Err(Error::CallerIsNotOwner);
+        }
+
+        let old_address = self.name_to_address.get(&name);
+        self.name_to_address.insert(name, new_address);
+
+        self.env().emit_event(Event::SetAddress(SetAddress {
+            name,
+            from: caller,
+            old_address,
+            new_address,
+        }));
+        Ok(())
+    }
+
+    /// Transfer owner to another address.
+    pub fn transfer(&mut self, name: Hash, to: AccountId) -> Result<()> {
+        let caller = self.env().caller();
+        let owner = self.get_owner_or_default(name);
+        if caller != owner {
+            return Err(Error::CallerIsNotOwner);
+        }
+
+        let old_owner = self.name_to_owner.get(&name);
+        self.name_to_owner.insert(name, to);
+
+        self.env().emit_event(Event::Transfer(Transfer {
+            name,
+            from: caller,
+            old_owner,
+            new_owner: to,
+        }));
+
+        Ok(())
+    }
+
+    /// Get address for specific name.
+    pub fn get_address(&self, name: Hash) -> AccountId {
+        self.get_address_or_default(name)
+    }
+
+    /// Get owner of specific name.
+    pub fn get_owner(&self, name: Hash) -> AccountId {
+        self.get_owner_or_default(name)
+    }
+
+    /// Returns the owner given the hash or the default address.
+    fn get_owner_or_default(&self, name: Hash) -> AccountId {
+        self.name_to_owner
+            .get(&name)
+            .unwrap_or(self.default_address)
+    }
+
+    /// Returns the address given the hash or the default address.
+    fn get_address_or_default(&self, name: Hash) -> AccountId {
+        self.name_to_address
+            .get(&name)
+            .unwrap_or(self.default_address)
+    }
+}
+
+/// Helper for referencing the zero address (`0x00`). Note that in practice this
+/// address should not be treated in any special way (such as a default
+/// placeholder) since it has a known private key.
+fn zero_address() -> AccountId {
+    [0u8; 32].into()
+}
