examples/ink_contracts/e2e_call_runtime.rs
@@ -1,0 +1,35 @@
+#[derive(Default, Clone, Copy)]
+struct AccountId(u128);
+
+type Balance = u128;
+
+struct Env {
+    caller: AccountId,
+}
+
+impl Env {
+    fn balance(&self) -> Balance {
+        unimplemented!()
+    }
+}
+
+#[derive(Default)]
+pub struct Contract {}
+
+impl Contract {
+    fn init_env() -> Env {
+        unimplemented!()
+    }
+
+    fn env(&self) -> Env {
+        Self::init_env()
+    }
+
+    pub fn new() -> Self {
+        Self {}
+    }
+
+    pub fn get_contract_balance(&self) -> Balance {
+        self.env().balance()
+    }
+}
