examples/ink_contracts/flipper.rs
@@ -1,0 +1,25 @@
+pub struct Flipper {
+    value: bool,
+}
+
+impl Flipper {
+    /// Creates a new flipper smart contract initialized with the given value.
+    pub fn new(init_value: bool) -> Self {
+        Self { value: init_value }
+    }
+
+    /// Creates a new flipper smart contract initialized to `false`.
+    pub fn new_default() -> Self {
+        Self::new(Default::default())
+    }
+
+    /// Flips the current value of the Flipper's boolean.
+    pub fn flip(&mut self) {
+        self.value = !self.value;
+    }
+
+    /// Returns the current value of the Flipper's boolean.
+    pub fn get(&self) -> bool {
+        self.value
+    }
+}
