examples/ink_contracts/lang_err_integration_tests/contract_ref.rs
@@ -1,0 +1,110 @@
+#[derive(Default, Clone, Copy)]
+struct AccountId(u128);
+
+type Balance = u128;
+
+type Hash = [u8; 32];
+
+struct Env {
+    caller: AccountId,
+}
+
+pub struct FlipperRef {
+    value: bool,
+}
+
+#[derive(Debug)]
+pub struct FlipperError;
+
+impl FlipperRef {
+    fn init_env() -> Env {
+        unimplemented!()
+    }
+
+    fn env(&self) -> Env {
+        Self::init_env()
+    }
+
+    /// Creates a new integration_flipper smart contract initialized with the given
+    /// value.
+    pub fn new(init_value: bool) -> Self {
+        Self { value: init_value }
+    }
+
+    /// Creates a new integration_flipper smart contract initialized to `false`.
+    pub fn new_default() -> Self {
+        Self::new(Default::default())
+    }
+
+    /// Attemps to create a new integration_flipper smart contract initialized with
+    /// the given value.
+    pub fn try_new(succeed: bool) -> Result<Self, FlipperError> {
+        if succeed {
+            Ok(Self::new(true))
+        } else {
+            Err(FlipperError)
+        }
+    }
+
+    pub fn flip(&mut self) {
+        self.value = !self.value;
+    }
+
+    pub fn get(&self) -> bool {
+        self.value
+    }
+}
+
+pub struct ContractRef {
+    flipper: FlipperRef,
+}
+
+impl ContractRef {
+    pub fn new(version: u32, flipper_code_hash: Hash) -> Self {
+        let salt = version.to_le_bytes();
+        let flipper = FlipperRef::new_default();
+        // .endowment(0)
+        // .code_hash(flipper_code_hash)
+        // .salt_bytes(salt)
+        // .instantiate();
+
+        Self { flipper }
+    }
+
+    pub fn try_new(version: u32, flipper_code_hash: Hash, succeed: bool) -> Self {
+        let salt = version.to_le_bytes();
+        let flipper = FlipperRef::try_new(succeed).unwrap();
+        // .endowment(0)
+        // .code_hash(flipper_code_hash)
+        // .salt_bytes(salt)
+        // .instantiate()
+        // .unwrap_or_else(|error| {
+        //     panic!(
+        //         "Received an error from the Flipper constructor while instantiating \
+        //              Flipper {error:?}"
+        //     )
+        // });
+
+        Self { flipper }
+    }
+
+    pub fn flip(&mut self) {
+        self.flipper.flip();
+    }
+
+    // pub fn flip_check(&mut self) {
+    //     self.flipper
+    //         .try_flip()
+    //         .expect("The ink! codegen should've produced a valid call.");
+    // }
+
+    pub fn get(&mut self) -> bool {
+        self.flipper.get()
+    }
+
+    // pub fn get_check(&mut self) -> bool {
+    //     self.flipper
+    //         .try_get()
+    //         .expect("The ink! codegen should've produced a valid call.")
+    // }
+}
